\documentclass[a4paper,10pt]{article}
\usepackage[utf8]{inputenc}

%opening
\title{}
\author{}

\usepackage{amsmath,amssymb,amsfonts,amsthm,mathtools} % Mathematik

\usepackage{color}

\begin{document}

\section*{Task 7}

\noindent Gauss Legendre quadrature is a quadrature rule where the evaluation points are the roots of the
$n$-th Legendre polynomial and the weights are the integrals of the corresponding Lagrange polynomials of degree $n$ over the integration domain.\\

\noindent Legendre polynomial:
\begin{align*}
 P_n(x)&=\frac{1}{2^n}\sum_{k=0}^n {n \choose k}^2 (x-1)^{n-k}(x+1)^k \\
 &= \sum_{k=0}^n {n \choose k}{-n-1 \choose k}\left(\frac{1-x}{2}\right)^k
\end{align*}

\noindent Lagrange polynomials:
\begin{align*}
 L_{i,n}(x)=\prod_{j=0 \atop j\neq i}^n \frac{x-x_j}{x_i-x_j}
\end{align*}
(Where $x_i$ are the evaluation points.)

% \noindent To proof:
% \begin{align*}
%  \frac{1}{\sqrt{2 \pi}} \int_{-\infty}^\infty f(s)e^{-\frac{s^2}{2}}ds =& \int_{0}^1 f(\Phi^{-1}(t))dt
% \end{align*}
% Proof:
% \begin{align*}
%  \frac{1}{\sqrt{2 \pi}} \int_{-\infty}^\infty f(s)e^{-\frac{s^2}{2}}ds =& \lim_{a\rightarrow \infty}\int_{-a}^a f(s) \phi '(s)ds\\
%   =& \lim_{a\rightarrow \infty}\int_{\Phi(-a)}^{\Phi(a)} f(\Phi^{-1}(t)) dt\\
%   =& \int_{0}^{1} f(\Phi^{-1}(t)) dt
% \end{align*}
% With substitution $s\rightarrow \Phi^{-1}(t)$.
% \flushright{$\qed$}


\end{document}
